Clap.lean
@@ -5,3 +5,4 @@ import Clap.Id
 import Clap.Cfold
 import Clap.Unshare
 import Clap.Dedup
+import Clap.Parser
