Clap/Parser.lean
@@ -1,0 +1,88 @@
+import Clap.Circuit
+import Clap.Simulation
+
+namespace Clap
+
+variable (F var:Type) [Field F] [DecidableEq F]
+
+def eq0 (e:F) : Option Unit :=
+  if e = 0 then some () else none
+
+def share (e:F) : F := e
+
+def is_zero (e:F) : F := if e = 0 then 1 else 0
+
+def accept : Unit -> Unit := fun () => ()
+
+/-
+  A circuit is a function from any number of F arguments to Option Unit.
+-/
+
+def ex (i:F) : Option Unit := do
+  eq0 F i
+  let vi <- share F i
+  eq0 F (vi + i)
+  accept ()
+
+-- def ex_unfolded : F -> Option Unit :=
+--   fun i =>
+--   bind (eq0 F i) (fun () =>
+--   bind (share F i) (fun vi =>
+--   bind (eq0 F (vi + i)) (fun () =>
+--   some ())))
+
+def ex_circuit_fun : Circuit' F := fun _ =>
+  .lam (fun i =>
+  .eq0 (.v i) (
+  .share (.v i) (fun vi =>
+  .eq0 (.v vi + .v i) (
+  .nil))))
+
+lemma equiv_eq0 : ∀ (el:F) (er:Exp F F) (cl:Option Unit) (cr:Circuit F F),
+  el = Exp.eval er ->
+  Simulation.s_bisim cl (Circuit.eval cr) ->
+  Simulation.s_bisim (Option.bind (eq0 F el) (fun () => cl)) (Circuit.eval (.eq0 er cr)) := by
+  intro el er cl cr he hc
+  simp only [Circuit.eval,Option.bind,eq0]
+  split
+  split
+  case _ _ heq her =>
+    rw [her] at he
+    rw [he] at heq
+    simp at heq
+  case _ _ hel her =>
+    constructor
+  case _ _ _ hel =>
+    simp at hel
+    rw [he] at hel
+    simp
+    split
+    . apply hc
+    . contradiction
+
+lemma equiv_share : ∀ (el:F) (er:Exp F F) (kl:F -> Option Unit) (kr:F -> Circuit F F),
+  el = Exp.eval er ->
+  (∀ x, Simulation.s_bisim (kl x) (Circuit.eval (kr x))) ->
+  Simulation.s_bisim (bind (share F el) kl) (Circuit.eval (.share er kr)) := by
+  intro el er kl kr he hk
+  simp only [Circuit.eval,bind,share]
+  rw [he]
+  apply hk
+
+theorem equiv : Simulation.s_bisim (ex F) (Circuit.eval' (ex_circuit_fun F)) := by
+  unfold ex_circuit_fun
+  unfold ex
+  simp only [bind]
+  simp only [Circuit.eval']
+  constructor
+  intro x
+  apply equiv_eq0
+  simp [Exp.eval]
+  apply equiv_share
+  simp [Exp.eval]
+  intro
+  apply equiv_eq0
+  simp [Exp.eval]
+  constructor
+
+end Clap
